NLustreToSyBloc/Translation.v
@@ -44,34 +44,6 @@ Module Type TRANSLATION
     fold_left gather_eq eqs ([], []).
 
 
-  (* XXX: computationally, the following [gather_*] are useless: they
-     are only used to simplify the proofs. See [gather_eqs_fst_spec]
-     and [gather_eqs_snd_spec]. *)
-
-  (* Definition gather_mem (eqs: list equation): idents := *)
-  (*   concatMap (fun eq => match eq with *)
-  (*                     | EqDef _ _ _ *)
-  (*                     | EqApp _ _ _ _ _ => [] *)
-  (*                     | EqFby x _ _ _ => [x] *)
-  (*                     end) eqs. *)
-  (* Definition gather_insts (eqs: list equation): list (ident * ident) := *)
-  (*   concatMap (fun eq => match eq with *)
-  (*                     | EqDef _ _ _ *)
-  (*                     | EqFby _ _ _ _ => [] *)
-  (*                     | EqApp i _ f _ _ => *)
-  (*                       match i with *)
-  (*                       | [] => [] *)
-  (*                       | i :: _ => [(i,f)] *)
-  (*                       end *)
-  (*                     end) eqs. *)
-  (* Definition gather_app_vars (eqs: list equation): idents := *)
-  (*   concatMap (fun eq => match eq with *)
-  (*                     | EqDef _ _ _ *)
-  (*                     | EqFby _ _ _ _ => [] *)
-  (*                     | EqApp xs _ _ _ _ => tl xs *)
-  (*                     end) eqs. *)
-
-
   (** ** Translation *)
 
   Definition translate_eqn (eqn: equation) : list SynSB.equation :=
@@ -83,7 +55,7 @@ Module Type TRANSLATION
     | EqApp xs ck f les None =>
       let s := hd Ids.default xs in
       [ SynSB.EqCall s xs ck false f les ]
-    | EqApp xs ck f les (Some (r, ck_r)) =>
+    | EqApp xs ck f les (Some r) =>
       let s := hd Ids.default xs in
       [ SynSB.EqReset s (Con ck r true) f;
           SynSB.EqCall s xs ck true f les ]
@@ -686,7 +658,7 @@ Module Type TRANSLATION
     - setoid_rewrite IHl; split; intros ** H.
       + right; auto.
       + inversion_clear H as [?? Hin|]; auto; inv Hin.
-    - destruct o as [[]|].
+    - destruct o as [|].
       + destruct i.
         * setoid_rewrite IHl; reflexivity.
         *{ setoid_rewrite In_snd_fold_left_gather_eq; split.
